hax-lib/proof-libs/fstar/core/Core_models.Result.fst
@@ -9,92 +9,94 @@ include Core_models.Bundle {Result_Ok as Result_Ok}
 
 include Core_models.Bundle {Result_Err as Result_Err}
 
-include Core_models.Bundle {impl__is_ok as impl__is_ok}
+include Core_models.Bundle {impl_1__is_ok as impl_1__is_ok}
 
-include Core_models.Bundle {impl__is_ok_and as impl__is_ok_and}
+include Core_models.Bundle {impl_1__is_ok_and as impl_1__is_ok_and}
 
-include Core_models.Bundle {impl__is_err as impl__is_err}
+include Core_models.Bundle {impl_1__is_err as impl_1__is_err}
 
-include Core_models.Bundle {impl__is_err_and as impl__is_err_and}
+include Core_models.Bundle {impl_1__is_err_and as impl_1__is_err_and}
 
-include Core_models.Bundle {impl__as_ref__from__result as impl__as_ref}
+include Core_models.Bundle {impl_1__as_ref as impl_1__as_ref}
 
-include Core_models.Bundle {impl__expect__from__result as impl__expect}
+include Core_models.Bundle {impl_1__expect as impl_1__expect}
 
-include Core_models.Bundle {impl__unwrap__from__result as impl__unwrap}
+include Core_models.Bundle {impl_1__unwrap as impl_1__unwrap}
 
-include Core_models.Bundle {impl__expect_err as impl__expect_err}
+include Core_models.Bundle {impl_1__expect_err as impl_1__expect_err}
 
-include Core_models.Bundle {impl__unwrap_err as impl__unwrap_err}
+include Core_models.Bundle {impl_1__unwrap_err as impl_1__unwrap_err}
 
-include Core_models.Bundle {impl__unwrap_or_else__from__result as impl__unwrap_or_else}
+include Core_models.Bundle {impl_1__unwrap_or_else as impl_1__unwrap_or_else}
 
-include Core_models.Bundle {impl__unwrap_or_default__from__result as impl__unwrap_or_default}
+include Core_models.Bundle {impl_1__unwrap_or_default as impl_1__unwrap_or_default}
 
-include Core_models.Bundle {impl__map__from__result as impl__map}
+include Core_models.Bundle {impl_1__map as impl_1__map}
 
-include Core_models.Bundle {impl__map_or__from__result as impl__map_or}
+include Core_models.Bundle {impl_1__map_or as impl_1__map_or}
 
-include Core_models.Bundle {impl__map_or_else__from__result as impl__map_or_else}
+include Core_models.Bundle {impl_1__map_or_else as impl_1__map_or_else}
 
-include Core_models.Bundle {impl__map_or_default__from__result as impl__map_or_default}
+include Core_models.Bundle {impl_1__map_or_default as impl_1__map_or_default}
 
-include Core_models.Bundle {impl__inspect__from__result as impl__inspect}
+include Core_models.Bundle {impl_1__inspect as impl_1__inspect}
 
-include Core_models.Bundle {impl__inspect_err as impl__inspect_err}
+include Core_models.Bundle {impl_1__inspect_err as impl_1__inspect_err}
 
-include Core_models.Bundle {impl__ok as impl__ok}
+include Core_models.Bundle {impl_1__ok as impl_1__ok}
 
-include Core_models.Bundle {impl__err as impl__err}
+include Core_models.Bundle {impl_1__err as impl_1__err}
 
-include Core_models.Bundle {impl__and__from__result as impl__and}
+include Core_models.Bundle {impl_1__and as impl_1__and}
 
-include Core_models.Bundle {impl__and_then__from__result as impl__and_then}
+include Core_models.Bundle {impl_1__and_then as impl_1__and_then}
 
-include Core_models.Bundle {impl__or__from__result as impl__or}
+include Core_models.Bundle {impl_1__or as impl_1__or}
 
-include Core_models.Bundle {impl__or_else__from__result as impl__or_else}
+include Core_models.Bundle {impl_1__or_else as impl_1__or_else}
 
-include Core_models.Bundle {impl__unwrap_or__from__result as impl__unwrap_or}
+include Core_models.Bundle {impl_1__unwrap_or as impl_1__unwrap_or}
 
-include Core_models.Bundle {impl__map_err as impl__map_err}
+include Core_models.Bundle {impl_1__map_err as impl_1__map_err}
 
-include Core_models.Bundle {impl__unwrap_unchecked__from__result as impl__unwrap_unchecked}
+include Core_models.Bundle {impl_1__unwrap_unchecked as impl_1__unwrap_unchecked}
 
-include Core_models.Bundle {impl__unwrap_err_unchecked as impl__unwrap_err_unchecked}
+include Core_models.Bundle {impl_1__unwrap_err_unchecked as impl_1__unwrap_err_unchecked}
 
-include Core_models.Bundle {impl__iter__from__result as impl__iter}
+include Core_models.Bundle {impl_1__iter as impl_1__iter}
 
-include Core_models.Bundle {impl_1__cloned__from__result as impl_1__cloned}
+include Core_models.Bundle {impl_2__cloned as impl_2__cloned}
 
-include Core_models.Bundle {impl_2__transpose as impl_2__transpose}
+include Core_models.Bundle {impl_3__transpose as impl_3__transpose}
 
-include Core_models.Bundle {impl_3__flatten as impl_3__flatten}
-
-include Core_models.Bundle {impl_4__from__result as impl_4}
+include Core_models.Bundle {impl_4__flatten as impl_4__flatten}
 
 include Core_models.Bundle {impl_5__from__result as impl_5}
 
 include Core_models.Bundle {impl_6__from__result as impl_6}
 
+include Core_models.Bundle {impl__from__result as impl}
+
+include Core_models.Bundle {impl_7__from__result as impl_7}
+
 include Core_models.Bundle {t_Iter__from__result as t_Iter}
 
 include Core_models.Bundle {Iter__from__result as Iter}
 
-include Core_models.Bundle {impl_7__from__result as impl_7}
+include Core_models.Bundle {impl_8__from__result as impl_8}
 
 include Core_models.Bundle {t_IntoIter__from__result as t_IntoIter}
 
 include Core_models.Bundle {IntoIter__from__result as IntoIter}
 
-include Core_models.Bundle {impl_9__from__result as impl_9}
-
 include Core_models.Bundle {impl_10__from__result as impl_10}
 
-include Core_models.Bundle {impl_11__as_deref as impl_11__as_deref}
+include Core_models.Bundle {impl_11__from__result as impl_11}
 
-include Core_models.Bundle {impl_13__copied as impl_13__copied}
+include Core_models.Bundle {impl_12__as_deref as impl_12__as_deref}
 
-include Core_models.Bundle {impl_14__into_ok as impl_14__into_ok}
+include Core_models.Bundle {impl_14__copied as impl_14__copied}
 
-include Core_models.Bundle {impl_15__into_err as impl_15__into_err}
+include Core_models.Bundle {impl_15__into_ok as impl_15__into_ok}
+
+include Core_models.Bundle {impl_16__into_err as impl_16__into_err}
